makefile
@@ -1,5 +1,5 @@
 
-default: src/SmtenIO.vo
+default: src/SmtenIO.vo src/SmtenS.vo
 
 %.vo: %.v
 	coqc -I lib -I src $<
@@ -9,6 +9,8 @@ lib/Smallstep.vo: lib/Imp.vo
 lib/Imp.vo: lib/SfLib.vo
 src/Smten.vo: lib/Types.vo
 src/SmtenProp.vo: src/Smten.vo
+src/SmtenS1.vo: src/SmtenProp.vo
+src/SmtenS.vo: src/SmtenS.vo
 src/SmtenIO.vo: src/SmtenProp.vo
 
 clean:
